Constr/CSet.v
@@ -1,7 +1,9 @@
-Require Export Setoid Coq.Classes.Morphisms.  
+Require Export Setoid Coq.Classes.Morphisms.
 Require Export Sets SetInterface SetConstructs SetProperties.
 Require Import EqDec Computable Util.
 Require Export CSetNotation CSetTac CSetBasic CSetCases CSetGet CSetComputable.
+
+Set Implicit Arguments.
 
 Lemma Proper_eq_fun X H0 (f:X->X)
 :  @Proper (X -> X)
@@ -16,11 +18,17 @@ Hint Resolve Proper_eq_fun.
 
 Hint Resolve incl_empty minus_incl incl_right incl_left : auto.
 
-(* 
+Definition pe X `{OrderedType X} := prod_eq (@Equal X _ _) (@Equal X _ _).
+
+Instance pe_morphism X `{OrderedType X}
+ : Proper (Equal ==> Equal ==> (@pe X _)) pair.
+Proof.
+  unfold Proper, respectful.
+  intros. econstructor; eauto.
+Qed.
+
+(*
 *** Local Variables: ***
 *** coq-load-path: (("../" "Lvc")) ***
 *** End: ***
 *)
-
-
-
